compiler/backend/clos_to_bvlScript.sml
@@ -69,6 +69,53 @@ Proof
   EVAL_TAC >> rw[] >> simp[]
 QED
 
+(* Constant flattening *)
+
+Overload PRIME[local] = “999983:num”;
+
+Definition part_hash_def:
+  part_hash (Int i) = Num (ABS i) MOD PRIME ∧
+  part_hash (Str s) = (LENGTH s + 3 * SUM (MAP ORD s)) MOD PRIME ∧
+  part_hash (W64 w) = (17 + w2n w) MOD PRIME ∧
+  part_hash (Con t ns) = (18 + 5 * t + 7 * SUM ns) MOD PRIME
+End
+
+Definition add_part_def:
+  add_part n p aux acc =
+    let h = part_hash p in
+      dtcase lookup h aux of
+      | NONE => (n+1n,n,insert h [(p,n)] aux,p::acc)
+      | SOME bucket =>
+          dtcase ALOOKUP bucket p of
+          | NONE => (n+1n,n,insert h ((p,n)::bucket) aux,p::acc)
+          | SOME k => (n,k,aux,acc)
+End
+
+Definition add_parts_def:
+  add_parts (ConstInt i) n aux acc = add_part n (Int i) aux acc ∧
+  add_parts (ConstStr s) n aux acc = add_part n (Str s) aux acc ∧
+  add_parts (ConstWord64 w) n aux acc = add_part n (W64 w) aux acc ∧
+  add_parts (ConstCons t cs) n aux acc =
+    (let (n, rs, aux, acc) = add_parts_list cs n aux acc in
+       add_part n (Con t rs) aux acc) ∧
+  add_parts_list [] n aux acc = (n,[],aux,acc) ∧
+  add_parts_list (c::cs) n aux acc =
+    let (n,r,aux,acc) = add_parts c n aux acc in
+    let (n,rs,aux,acc) = add_parts_list cs n aux acc in
+      (n,r::rs,aux,acc)
+End
+
+Definition const_to_parts_def:
+  const_to_parts (ConstInt i) = [Int i] ∧
+  const_to_parts (ConstStr s) = [Str s] ∧
+  const_to_parts (ConstWord64 w) = [W64 w] ∧
+  const_to_parts (ConstCons t cs) =
+    let (n, rs, aux, acc) = add_parts_list cs 0 LN [] in
+      REVERSE ((Con t rs)::acc)
+End
+
+(* / Constant flattening *)
+
 val num_added_globals_def = Define
   `num_added_globals = 1n`;
 
@@ -85,6 +132,7 @@ val compile_op_def = Define`
   compile_op DerefByteVec = DerefByte ∧
   compile_op (SetGlobal n) = SetGlobal (n + num_added_globals) ∧
   compile_op (Global n) = Global (n + num_added_globals) ∧
+  compile_op (Constant c) = Build (const_to_parts c) ∧
   compile_op x = x`
 val _ = export_rewrites["compile_op_def"];
 
@@ -101,6 +149,7 @@ Theorem compile_op_pmatch:
       | DerefByteVec => DerefByte
       | SetGlobal n => SetGlobal (n + num_added_globals)
       | Global n => Global (n + num_added_globals)
+      | Constant c => Build (const_to_parts c)
       | x => x
 Proof
   rpt strip_tac
